rupicola/io/IO.fsti
@@ -8,7 +8,7 @@ module IO
     do notation. **)
 
 include BaseTypes
-open Hist
+include Hist
 open Trace
 open FStar.List.Tot
 
@@ -28,27 +28,27 @@ val write (x:bool) : io (resexn unit)
 
 val theta : #a:Type -> io a -> hist a
 
-val io_bind_equivalence #a #b (k k':a -> io b) (m:io a) (h:history) :
+val io_bind_equivalence #a #b (k k':a -> io b) (m:io a) :
   Lemma (requires forall x. k x == k' x)
-        (ensures forall p. theta (io_bind m k) h p == theta (io_bind m k') h p)
+        (ensures theta (io_bind m k) `hist_equiv` theta (io_bind m k'))
 
 let return = io_return
 let (let!@) = io_bind
 
 val lem_theta_return #a (x:a) (h:history) (lt:local_trace h) :
   Lemma (requires lt == [])
-        (ensures forall p. theta (return x) h p ==> p lt x)
+        (ensures wp2p (theta (return x)) h lt x)
 
 val lem_theta_bind #a #b (m:io a) (h:history) (lt2:local_trace h) (fs_r_m:a) (k:a -> io b) (lt3:local_trace (h++lt2)) (fs_r:b) (lt:local_trace h) :
-  Lemma (requires (forall (p:hist_post h a). theta m h p ==> p lt2 fs_r_m) /\
-                  (forall (p':hist_post (h++lt2) b). theta (k fs_r_m) (h++lt2) p' ==> p' lt3 fs_r) /\
+  Lemma (requires wp2p (theta m) h lt2 fs_r_m /\
+                  wp2p (theta (k fs_r_m)) (h++lt2) lt3 fs_r /\
                   (lt == lt2 @ lt3))
-        (ensures forall (p_:hist_post h b). theta (io_bind m k) h p_ ==> p_ lt fs_r)
+        (ensures wp2p (theta (io_bind m k)) h lt fs_r)
 // theta (io_bind m k) == pred transformer bind of (theta m) (fun x -> theta (k x))
 
 val theta_history_independence #a (m:io a) (h:history) (lt:local_trace h) (fs_r:a) :
-  Lemma (requires forall p. theta m h p ==> p lt fs_r)
-        (ensures forall h' (lt':local_trace h') p'. theta m h' p' ==> p' lt' fs_r) // use steps e e' h lt and construct_local_trace
+  Lemma (requires wp2p (theta m) h lt fs_r)
+        (ensures forall h' (lt':local_trace h'). wp2p (theta m) h' lt' fs_r) // use steps e e' h lt and construct_local_trace
 
 val theta_history_independence' (#a:Type) (m:io a) (h:history) (p:hist_post h a) :
   Lemma (requires theta m h p)
