rupicola/io/RrHP.fst
@@ -34,32 +34,32 @@ let linkS (#i:intS) (ps:progS i) (cs:ctxS i) : wholeS =
   (dfst ps) cs
 
 (** Definition from SCIO*, section 6.2 **)
-type behS_t = local_trace [] * bool -> Type0
+type behS_t = hist_post [] bool
 val behS : wholeS -> behS_t
-let behS ws = fun (lt, res) -> forall p. theta ws [] p ==> p lt res
+let behS ws = wp2p (theta ws) []
 
 (** Target **)
 // right now, we give the target a source type (which might have pre post conditions, etc.) -> which is not a correct model of unverified code
 // unverified code: target + target type (typ)
 // but maybe current typing works? cause you cannot have pre post conditions
 // the type of target contexts restricts us to unverified code
-  noeq type intT = { ct : qType }
+noeq type intT = { ct : qType }
 
-  val comp_int : intS -> intT
-  //let comp_int i = { ct = type_quotation_to_typ i.qct }
-  let comp_int i = { ct = i.ct }
+val comp_int : intS -> intT
+//let comp_int i = { ct = type_quotation_to_typ i.qct }
+let comp_int i = { ct = i.ct }
 
-  type progT (i:intT) = closed_exp
+type progT (i:intT) = closed_exp
 
-  // the typing makes sure that there are no pre post conditions - maybe...
-  type ctxT (i:intT) = ct:value & typing empty ct i.ct
-  (** syntactic typing necessary to be able to backtranslate **)
-  type wholeT = closed_exp
+// the typing makes sure that there are no pre post conditions - maybe...
+type ctxT (i:intT) = ct:value & typing empty ct i.ct
+(** syntactic typing necessary to be able to backtranslate **)
+type wholeT = closed_exp
 
-  let linkT (#i:intT) (pt:progT i) (ct:ctxT i) : wholeT =
-    let (| e, h |) = ct in
-    let wt = EApp pt e in
-    wt
+let linkT (#i:intT) (pt:progT i) (ct:ctxT i) : wholeT =
+  let (| e, h |) = ct in
+  let wt = EApp pt e in
+  wt
 
 let compile_prog (#i:intS) (ps:progS i) : progT (comp_int i) =
   compile_closed (dsnd ps)
@@ -74,8 +74,8 @@ let behT wt = fun (lt, r) -> steps wt r [] lt
 
 val rel_behs : behS_t -> behT_t -> Type0
 let rel_behs (bs:behS_t) (bt:behT_t) =
-  (forall rS lt. bs (lt, rS) ==>  (exists rT. rel_bools rS rT /\ bt (lt, rT))) /\
-  (forall rT lt. bt (lt, rT) ==>  (exists rS. rel_bools rS rT /\ bs (lt, rS)))
+  (forall rS lt. bs lt rS ==>  (exists rT. rel_bools rS rT /\ bt (lt, rT))) /\
+  (forall rT lt. bt (lt, rT) ==>  (exists rS. rel_bools rS rT /\ bs lt rS))
 
 let lem_rel_beh (fs_e:wholeS) (e:wholeT)
   : Lemma
